More WIP on informative parse

src/Parsers/ParserImplementationOptimized.v
@@ -19,56 +19,60 @@ Local Open Scope list_scope.
 
 Definition transfer_parser_keep_string {Char G} {HSLM HSL}
            (old : @Parser Char G HSLM HSL)
-           (new : @String Char HSLM -> bool)
-           (H : forall s, new s = has_parse old s)
+           (new_has_parse : @String Char HSLM -> _)
+           (new_parse : @String Char HSLM -> _)
+           (H_has_parse : forall s, new_has_parse s = has_parse old s)
+           (H_parse : forall s, new_parse s = parse old s)
 : @Parser Char G HSLM HSL.
 Proof.
-  refine {| has_parse := new;
-            parse := parse old |};
+  refine {| has_parse := new_has_parse;
+            parse := new_parse |};
   abstract (
       intros;
-      rewrite H in *;
+      rewrite ?H_has_parse, ?H_parse in *;
         first [ apply (has_parse_sound old); assumption
               | eapply (has_parse_complete old); eassumption
               | eapply (parse_correct old); eassumption ]
     ).
 Defined.
 
-Arguments transfer_parser_keep_string {_ _ _ _} _ _ _.
+Arguments transfer_parser_keep_string {_ _ _ _} _ _ _ _ _.
 
 Definition transfer_parser {Char G} {HSLM1 HSLM2 HSL1 HSL2}
            (old : @Parser Char G HSLM1 HSL1)
            (make_string : @String Char HSLM2 -> @String Char HSLM1)
-           (new : @String Char HSLM2 -> bool)
-           (H : forall s, new s = has_parse old (make_string s))
+           (new_has_parse : @String Char HSLM2 -> _)
+           (new_parse : @String Char HSLM2 -> _)
+           (H_has_parse : forall s, new_has_parse s = has_parse old (make_string s))
+           (H_parse : forall s, new_parse s = parse old (make_string s))
            (R : @String Char HSLM1 -> @String Char HSLM2 -> Prop)
            (R_make : forall str, R (make_string str) str)
            (R_respectful : transfer_respectful R)
            (R_flip_respectful : transfer_respectful (Basics.flip R))
 : @Parser Char G HSLM2 HSL2.
 Proof.
-  refine {| has_parse := new;
-            parse str := parse old (make_string str) |}.
+  refine {| has_parse := new_has_parse;
+            parse := new_parse |}.
   { abstract (
         intros str H';
-        rewrite H in H';
+        rewrite H_has_parse in H';
         refine (@transfer_parse_of_item Char _ _ _ _ G R R_respectful (make_string str) str (NonTerminal G) (R_make str) _);
         apply (has_parse_sound old); assumption
       ). }
   { abstract (
         intros str p;
-        rewrite H;
+        rewrite H_has_parse;
         pose (@transfer_parse_of_item Char _ _ _ _ G (Basics.flip R) R_flip_respectful str (make_string str) (NonTerminal G) (R_make str) p) as p';
         apply (has_parse_complete old p'); subst p';
         exact (transfer_forall_parse_of_item _ H')
       ). }
   { abstract (
         intros str;
-        rewrite H, parse_correct; reflexivity
+        rewrite H_has_parse, H_parse, parse_correct; reflexivity
       ). }
 Defined.
 
-Arguments transfer_parser {_ _ _ _ _ _} _ _ _ _ _ _ _ _.
+Arguments transfer_parser {_ _ _ _ _ _} _ _ _ _ _ _ _ _ _ _.
 
 Section implementation.
   Context {G : pregrammar Ascii.ascii}.
@@ -109,13 +113,18 @@ Section implementation.
     let implH := constr:(fun str => proj2_sig (impl0 str)) in
     let impl' := (eval cbv beta iota zeta delta [RDPList.rdp_list_remove_nonterminal RDPList.rdp_list_initial_nonterminals_data RDPList.rdp_list_nonterminals_listT RDPList.rdp_list_is_valid_nonterminal RDPList.rdp_list_ntl_wf RDPList.rdp_list_nonterminals_listT_R RDPList.rdp_list_of_nonterminal RDPList.rdp_list_to_nonterminal Carriers.default_nonterminal_carrierT Carriers.some_invalid_nonterminal Carriers.default_to_production Carriers.default_to_nonterminal] in impl) in
     let impl := (eval simpl in impl') in
+    let s_impl0 := constr:(fun str => SimpleRecognizer.parse_nonterminal (make_string str) (Start_symbol G)) in
+    let s_impl := (eval simpl in s_impl0) in
+    let s_impl := (eval cbv [SimpleRecognizer.parse_nonterminal SimpleRecognizer.parse_nonterminal' nonterminals_length initial_nonterminals_data predata pdata RDPList.rdp_list_predata RDPList.rdp_list_initial_nonterminals_data of_nonterminal RDPList.rdp_list_of_nonterminal SimpleRecognizer.parse_nonterminal_or_abort nonterminals_listT RDPList.rdp_list_nonterminals_listT default_nonterminal_carrierT nonterminal_carrierT SimpleRecognizer.parse_nonterminal_step SimpleRecognizer.parse_productions' nonterminal_to_production is_valid_nonterminal RDPList.rdp_list_is_valid_nonterminal remove_nonterminal RDPList.rdp_list_remove_nonterminal RDPList.rdp_list_nonterminal_to_production RDPList.rdp_list_to_nonterminal default_to_nonterminal SimpleRecognizer.option_simple_parse_of_orb SimpleRecognizer.parse_production' SimpleRecognizer.parse_production'_for SimpleRecognizer.option_orb SimpleRecognizer.option_SimpleParseProductionCons SimpleRecognizer.parse_item'] in s_impl) in
     refine (transfer_parser
               (HSL1 := splitter) (HSL2 := stringlike_stringlike)
               (parser splitter Hvalid) make_string
               impl
+              s_impl
               (fun str => eq_trans
                             (implH str)
                             (@parse_nonterminal_proj _ splitter string_like_min_lite G pdata' _ _ _ HSLPr _ _))
+              (fun str => eq_refl : s_impl0 str = SimpleRecognizer.parse_nonterminal (make_string str) G)
               R R_make _ _).
   Defined.
 
